$$\sum^{h \text{ (End Index)}}_{k=1\text{ (Starting Index)}} a_x$$
# Rules for finite sum
1. Sum Rule$$\sum^{n}_{k=1} a_k+b_k=\sum^{n}_{k=1} a_k+\sum^{n}_{k=1} b_k$$
2. Difference Rule $$\sum^{n}_{k=1}a_k+b_k=\sum^{n}_{k=1}a_k-\sum^{n}_{k=1}b_k$$
3. Constant Multiple Rule $$\sum^{n}_{k=1}c \text{ (Constant)}*a_k=\sum^{n}_{k=1}a_k$$
4. Constant Value Rule $$\sum^{n}_{k=1}c=n*c$$
#### Example
Rewrite $\sum^{n}_{k=1}(3k-k^2)$ 
> $$\sum^{n}_{k=1}3k-\sum^{n}_{k=1}k^2$$
> $$3\sum^{n}_{k=1}k-\sum^{n}_{k=1}k^2$$
## Important Summations
1. $$\sum^{n}_{k=1}c=c*n$$
2. $$\sum^{n}_{k=1}k=\frac{n(n+1)}{2}$$
3. $$\sum^{n}_{k=1}k^2=\frac{n(n+1)(2n+1)}{6}$$
4. $$\sum^{n}_{k=1}k^3=(\frac{n(n+1)}{2})^2$$
#### Example
Find $\sum^{7}_{k=1}k(2k+1)$
> $$\sum^{7}_{k=1}2k^2+k$$
> $$=\sum^{7}_{k=1}2k^2+\sum^{7}_{k=1}k$$
> $$=2\sum^{7}_{k=1}k^2+\sum^{7}_{k=1}k$$
> $$=2(\frac{7(7+1)(2(7)+1)}{6})+\frac{7(7+1)}{2}$$
> $$=\frac{2(7)(8)(15)}{6}+\frac{7(8)}{2}$$
> $$=(35*8)+(7*4)$$
> $$=280+28$$
> $$=308$$